tactics.v
@@ -8,10 +8,10 @@ From cryptis Require Import lib term cryptis primitives.
 Import bi.
 Import env_notations.
 
-Global Hint Extern 1 (envs_entails _ (sterm _)) =>
-  iApply pterm_sterm : core.
-Global Hint Extern 0 (envs_entails _ (pterm (TInt ?n))) =>
-  rewrite (pterm_TInt n) : core.
+Global Hint Extern 1 (envs_entails _ (minted _)) =>
+  iApply public_minted : core.
+Global Hint Extern 0 (envs_entails _ (public (TInt ?n))) =>
+  rewrite (public_TInt n) : core.
 
 Section Proofs.
 
